Loom/Tactic/Match.lean
@@ -1,3 +1,8 @@
+/-
+Copyright (c) 2025 Lean FRO LLC. All rights reserved.
+Released under Apache 2.0 license as described in the file LICENSE.
+Authors: Vladimir Gladshtein, Sebastian Graf
+-/
 import Lean
 import Loom.Tactic.Attr
 import Loom.Tactic.Spec
